Garden/Plonky3/keccak/air_local.v
@@ -1,0 +1,143 @@
+Require Import Garden.Plonky3.M.
+Require Import Garden.Plonky3.keccak.air_small_parts.
+Require Import Garden.Plonky3.keccak.columns.
+Require Import Garden.Plonky3.keccak.constants.
+
+(** In this definition, we group all the constraints about the current [local] row. *)
+Definition eval_local {p} `{Prime p} (local : KeccakCols.t) : M.t unit :=
+  let* _ := eval_preimage_a local in
+  let* _ := eval_assert_export_bool local in
+  let* _ := eval_assert_export_zero local in
+  let* _ := eval_assert_c_c_prime local in
+  let* _ := eval_assert_a_a_prime_c_c_prime local in
+  let* _ := eval_assert_a_prime_c_prime local in
+  let* _ := eval_assert_a_prime_prime local in
+  let* _ := eval_assert_a_prime_prime_0_0_bits_bools local in
+  let* _ := eval_assert_a_prime_prime_0_0_limbs local in
+  let* _ := eval_assert_a_prime_prime_prime_0_0_limbs local in
+  M.pure tt.
+
+Module KeccakCols.
+  Definition get_a (local : KeccakCols.t) (y x z : Z) : bool :=
+    Limbs.get_bit BITS_PER_LIMB ((local.(KeccakCols.a).(Array.get) y).(Array.get) x) z.
+
+  Definition get_c (local : KeccakCols.t) (x z : Z) : bool :=
+    Z.odd ((local.(KeccakCols.c).(Array.get) x).(Array.get) z).
+
+  Definition get_c_prime (local : KeccakCols.t) (x z : Z) : bool :=
+    Z.odd ((local.(KeccakCols.c_prime).(Array.get) x).(Array.get) z).
+
+  Definition get_a_prime (local : KeccakCols.t) (y x z : Z) : bool :=
+    Z.odd (((local.(KeccakCols.a_prime).(Array.get) y).(Array.get) x).(Array.get) z).
+End KeccakCols.
+
+Definition xorbs (bs : list bool) : bool :=
+  Lists.List.fold_left xorb bs false.
+
+Module FirstRowsFrom_a.
+  Module From.
+    Record t (local : KeccakCols.t) : Set := {
+      c_c_prime (x z : Z) :
+        KeccakCols.get_c_prime local x z =
+        xorbs [
+          KeccakCols.get_c local x z;
+          KeccakCols.get_c local ((x + 4) mod 5) z;
+          KeccakCols.get_c local ((x + 1) mod 5) ((z + 63) mod 64)
+        ];
+      a_a_prime_c_c_prime (x y z : Z) :
+        KeccakCols.get_a local x y z =
+        xorbs [
+          KeccakCols.get_a_prime local x y z;
+          KeccakCols.get_c local x z;
+          KeccakCols.get_c_prime local x z
+        ];
+      a_prime_c_prime (x z : Z) :
+        KeccakCols.get_c_prime local x z =
+        xorbs [
+          KeccakCols.get_a_prime local x 0 z;
+          KeccakCols.get_a_prime local x 1 z;
+          KeccakCols.get_a_prime local x 2 z;
+          KeccakCols.get_a_prime local x 3 z;
+          KeccakCols.get_a_prime local x 4 z
+        ];
+    }.
+  End From.
+
+  Module To.
+    Record t (local : KeccakCols.t) : Set := {
+      a_c (x z : Z) :
+        KeccakCols.get_c local x z =
+        xorbs [
+          KeccakCols.get_a local x 0 z;
+          KeccakCols.get_a local x 1 z;
+          KeccakCols.get_a local x 2 z;
+          KeccakCols.get_a local x 3 z;
+          KeccakCols.get_a local x 4 z
+        ];
+      c_c_prime (x z : Z) :
+        KeccakCols.get_c_prime local x z =
+        xorbs [
+          KeccakCols.get_c local x z;
+          KeccakCols.get_c local ((x + 4) mod 5) z;
+          KeccakCols.get_c local ((x + 1) mod 5) ((z + 63) mod 64)
+        ];
+      a_a_prime_c (x y z : Z) :
+        KeccakCols.get_a_prime local x y z =
+        xorbs [
+          KeccakCols.get_a local x y z;
+          KeccakCols.get_c local ((x + 4) mod 5) z;
+          KeccakCols.get_c local ((x + 1) mod 5) ((z + 63) mod 64)
+        ];
+    }.
+  End To.
+
+  (** The lemma explains why the calculation for the first rows is deterministic. *)
+  Lemma from_implies_to (local : KeccakCols.t) :
+    From.t local ->
+    To.t local.
+  Proof.
+    intros []; constructor; intros; cbn in *.
+    { repeat rewrite a_a_prime_c_c_prime.
+      repeat rewrite a_prime_c_prime.
+      repeat destruct (KeccakCols.get_c _);
+        repeat destruct (KeccakCols.get_a_prime _);
+        reflexivity.
+    }
+    { congruence. }
+    { rewrite a_a_prime_c_c_prime.
+      rewrite c_c_prime.
+      repeat destruct (KeccakCols.get_a_prime _);
+        repeat destruct (KeccakCols.get_c _);
+        reflexivity.
+    }
+  Qed.
+End FirstRowsFrom_a.
+
+(** Lemma to show that the calculation with the [diff] is actually a calculation of XOR. *)
+Lemma xor_sum_diff_eq (local : KeccakCols.t) (x z : Z)
+  (H_sum_diff :
+    let diff :=
+      Lists.List.fold_left Z.add [
+        Z.b2z (KeccakCols.get_a_prime local x 0 z);
+        Z.b2z (KeccakCols.get_a_prime local x 1 z);
+        Z.b2z (KeccakCols.get_a_prime local x 2 z);
+        Z.b2z (KeccakCols.get_a_prime local x 3 z);
+        Z.b2z (KeccakCols.get_a_prime local x 4 z)
+      ] 0 -
+      Z.b2z (KeccakCols.get_c_prime local x z) in
+    diff = 0 \/ diff = 2 \/ diff = 4
+  ) :
+  KeccakCols.get_c_prime local x z =
+  xorbs [
+    KeccakCols.get_a_prime local x 0 z;
+    KeccakCols.get_a_prime local x 1 z;
+    KeccakCols.get_a_prime local x 2 z;
+    KeccakCols.get_a_prime local x 3 z;
+    KeccakCols.get_a_prime local x 4 z
+  ].
+Proof.
+  destruct (KeccakCols.get_c_prime _);
+    repeat destruct (KeccakCols.get_a_prime _);
+    cbn in *;
+    lia.
+Qed.
